\begin{enumerate}[label=\thesection.\arabic*.,ref=\thesection.\theenumi]
\numberwithin{equation}{enumi}
\item Let the state-space representation of an LTI system be
\begin{align}
\dot{\vec{x}(t)}&=\vec{A}\vec{x}(t)+\vec{B}\vec{u}(t) \\
 \vec{y}(t)&=\vec{C}\vec{x}(t)+D u(t)
\end{align}
A,B,C are matrices, D is scalar, u(t) is input to the system and y(t) is output to the system. let
\begin{equation}
 b1 =\begin{vmatrix}
  0&0&1\\
 \end{vmatrix}
\end{equation}
\begin{align}
b1^T=B
\end{align}
and D=0. Find A and C.
\begin{align}
H(s)=\frac{1}{s^3+3s^2+2s+1}
\end{align}
\solution
\\ \textbf{FINDING TRANSFER FUNCTION}
\\so
\begin{align}
 \dot{X(t)}=AX(t)+BU(t) \\
 Y(t)=CX(t)+DU(t)
\end{align}    
\\by applying laplace transforms on both sides of equation 1
we get
\\s.X(s)-X(0)=A.X(s)+B.U(s)
\\s.X(s)-A.X(s)=B.U(s)+X(0)
\\(sI-A)X(s)=X(0)+B.U(s)
\\$X(s)=X(0)([sI-A])^{-1}+(([sI-A])^{-1}B)U(s)$
\\Laplace transform of equation 2 and sub X(s) 
\\Y(s)=C.X(s)+D.U(s)
\\$Y(s)=C.[X(0)([sI-A])^{-1 }+ (([sI-A])^{-1}B)U(s)]+DU(s)$
\\If X(0)=0
\\then $Y(s)=C[(([sI-A])^{-1}B)U(s)]+DU(s)$
\\$\frac{Y(s)}{U(s)}=C[(([sI-A])^{-1}B)]+D=H(s)$
\\
\\ As we know that
\\ $Y(s)=H(s) \times U(s)= (\frac{1}{s^3+3s^2+2s+1}) \times U(s) $
\\
\\ $H(s)=\frac{Y(s)}{U(s)}=(\frac{(\frac{Y(s)}{x_{1}(s)})}{\frac{U(s)}{x_{1}(s)}})=\frac{1}{s^3+3s^2+2s+1} $
\\
\\let   $x_{1}(s)=\frac{U(s)}{s^3+3s^2+2s+1}$
\\
\\$Y(s)=x_{1}(s)\times 1 $
\begin{align}
s^3x_{1}(s)+3s^2x_{1}(s)+2sx_{1}(s)+x_{1}(s)=U(s)
\end{align}
\\ Taking inverse laplace transform we get
\\$\dddot{x_{1}(t)}+\ddot{x_{1}(t)}+\dot{x_{1}(t)}+x_{1}(t)=U(t)$
\\$\dot{x_{1}}=x_{2}$
\\$\ddot{x_{1}}=\dot{x_{2}}=x_{3}$
\\$\dddot{x_{1}}=\ddot{x_{2}}=\dot{x_{3}}$
\\ so equation 1.1.4 can be written as
\\
\begin{gather}
\begin{bmatrix}
sx_{1}(s)\\
s^2x_{1}(s)\\
s^3x_{1}(s)
\end{bmatrix}
=
\begin{bmatrix}
0&1&0\\
0&0&1\\
-1&-2&-3
\end{bmatrix}\times \begin{bmatrix}
x_{1}(s)\\
sx_{1}(s)\\
s^2x{1}(s)
\end{bmatrix}
+
\begin{bmatrix}
0\\
0\\
1
\end{bmatrix} \times U
\end{gather}
taking inverse laplace transform
\begin{gather}
\begin{bmatrix}
\dot{x_{1}}\\
\dot{x_{2}}\\
\dot{x_{3}}
\end{bmatrix}
=
\begin{bmatrix}
0&1&0\\
0&0&1\\
-1&-2&-3
\end{bmatrix}\times \begin{bmatrix}
x_{1}\\
x_{2}\\
x_{3}
\end{bmatrix}
+
\begin{bmatrix}
0\\
0\\
1
\end{bmatrix} \times U
\end{gather}
therfore
\begin{equation}
A=\begin{bmatrix}
0&1&0\\
0&0&1\\
-1&-2&-3
\end{bmatrix}
\end{equation}
\\
Since $ Y(s)=x_{1}(s)\times numerator$
\\therefore $ Y(s)=x_{1}(s) $
\begin{gather}
\\Y=
\begin{bmatrix}
1&0&0
\end{bmatrix}\times \begin{bmatrix}
x_{1}(s)\\
sx_{1}(s)\\
s^2x_{1}(s)
\end{bmatrix} 
\end{gather}
taking inverse laplace transform
\begin{gather}
\\Y=
\begin{bmatrix}
1&0&0
\end{bmatrix}\times \begin{bmatrix}
x_{1}\\
x_{2}\\
x_{3}
\end{bmatrix} 
\end{gather}
\begin{equation}
C=\begin{bmatrix}
1&0&0
\end{bmatrix}
\end{equation}
%\end{document}

%\end{document}
\end{enumerate}

